fully introduce tiling in blocktiling2d, continue on tc

src/lib/poly/gemm/Kuiper.Poly.GEMM.BlockTiling2D.fst
@@ -25,7 +25,6 @@ open Kuiper.VArray {
   varray_pts_to,
   varray_pts_to_cell
 }
-open Kuiper.TensorCore
 open Kuiper.Matrix.Tiling
 
 (* Description of shared memory used in this kernel. *)
@@ -41,47 +40,48 @@ let shmems_desc
 
 unfold
 let bid_y
-  (rows cols : erased nat)
-  (bm : erased nat {bm > 0 /\ bm /? rows})
-  (bn : erased nat {bn > 0 /\ bn /? cols})
-  (bid : enatlt (rows/bm * (cols/bn)))
-  : enatlt (rows/bm)
+  (rows cols : nat)
+  (bm : nat {bm > 0 /\ bm /? rows})
+  (bn : nat {bn > 0 /\ bn /? cols})
+  (bid : natlt (rows/bm * (cols/bn)))
+  : natlt (rows/bm)
   =
     bid / (cols/bn)
 
 unfold
 let bid_x
-  (rows cols : erased nat)
-  (bm : erased nat {bm > 0 /\ bm /? rows})
-  (bn : erased nat {bn > 0 /\ bn /? cols})
-  (bid : enatlt (rows/bm * (cols/bn)))
-  : enatlt (cols/bn)
+  (rows cols : nat)
+  (bm : nat {bm > 0 /\ bm /? rows})
+  (bn : nat {bn > 0 /\ bn /? cols})
+  (bid : natlt (rows/bm * (cols/bn)))
+  : natlt (cols/bn)
   =
   bid % (cols/bn)
 
 unfold
 let tid_y
-  (bm bn : erased nat)
-  (tm : erased nat {tm > 0 /\ tm /? bm})
-  (tn : erased nat {tn > 0 /\ tn /? bn})
-  (tid : enatlt (bm/tm * (bn/tn)))
-  : enatlt (bm/tm)
+  (bm bn : nat)
+  (tm : nat {tm > 0 /\ tm /? bm})
+  (tn : nat {tn > 0 /\ tn /? bn})
+  (tid : natlt (bm/tm * (bn/tn)))
+  : natlt (bm/tm)
   =
     tid / (bn/tn)
 
 unfold
 let tid_x
-  (bm bn : erased nat)
-  (tm : erased nat {tm > 0 /\ tm /? bm})
-  (tn : erased nat {tn > 0 /\ tn /? bn})
-  (tid : enatlt (bm/tm * (bn/tn)))
-  : enatlt (bn/tn)
+  (bm bn : nat)
+  (tm : nat {tm > 0 /\ tm /? bm})
+  (tn : nat {tn > 0 /\ tn /? bn})
+  (tid : natlt (bm/tm * (bn/tn)))
+  : natlt (bn/tn)
   =
     tid % (bn/tn)
 
 inline_for_extraction noextract
 instance concrete_sz_1 : concrete_sz 1 = { x = 1sz }
 
+inline_for_extraction noextract
 let block_tile
   (#et : Type0) {| scalar et |}
   (#rows #cols : erased nat)
@@ -92,9 +92,11 @@ let block_tile
   (bid : enatlt (rows/bm * (cols/bn)))
   : gpu_matrix et
       (subtile_layout lC bm bn
-        (bid_y rows cols bm bn bid) (bid_x rows cols bm bn bid))
+        (bid_y rows cols (hide (SZ.v bm)) (hide (SZ.v bn)) bid)
+        (bid_x rows cols (hide (SZ.v bm)) (hide (SZ.v bn)) bid))
   =
-    gpu_matrix_subtile gC bm bn (bid_y rows cols bm bn bid) (bid_x rows cols bm bn bid)
+    gpu_matrix_subtile gC (hide (SZ.v bm)) (hide (SZ.v bn))
+      (bid_y rows cols bm bn bid) (bid_x rows cols bm bn bid)
 
 let thread_tile
   (#et : Type0) {| scalar et |}
@@ -108,7 +110,8 @@ let thread_tile
       (subtile_layout lC_bt tm tn
         (tid_y bm bn tm tn tid) (tid_x bm bn tm tn tid))
   =
-   gpu_matrix_subtile gC_bt tm tn (tid_y bm bn tm tn tid) (tid_x bm bn tm tn tid)
+   gpu_matrix_subtile gC_bt (hide (SZ.v tm)) (hide (SZ.v tn))
+    (tid_y bm bn tm tn tid) (tid_x bm bn tm tn tid)
 
 let own_thread_tile
   (#et : Type0) {| scalar et |}
@@ -194,12 +197,12 @@ let own_shmem_cell
 let div_ceil (a : erased nat) (b : pos) = (a + (b-1))/b
 let own_tile_stride_cells
   (#et : Type0)
-  (#rows #cols : erased nat)
+  (#rows #cols : nat)
   (#lm : mlayout rows cols)
   ([@@@mkey] m : gpu_matrix et lm)
   // (em : ematrix et rows cols)
-  (nthr : erased nat)
-  (tid : enatlt nthr)
+  (nthr : nat)
+  (tid : natlt nthr)
   : slprop
   =
   (* using enatlt here would require enumerable enatlt which is not entirely straightforward *)
@@ -408,7 +411,7 @@ fn populate_shmem
   (tile_row : szlt (rows/bm))
   (tile_shared : szlt (shared/bk))
   (tile_col : szlt (cols/bn))
-  (tid : szlt (bm/^tm *^ (bn/^tn)))
+  (tid : szlt (bm/tm * (bn/tn)))
   preserves
     gpu **
     (gA |-> Frac fA eA) **
@@ -417,10 +420,12 @@ fn populate_shmem
     own_tile_stride_cells sA (bm/tm * (bn/tn)) tid **
     own_tile_stride_cells sB (bm/tm * (bn/tn)) tid
 {
-  let tileA = gpu_matrix_extract_tile' gA bm bk tile_row tile_shared;
-  cp_matrix bm bk tileA sA (get_bdim()) tid;
+  let tileA = gpu_matrix_extract_tile_ro' gA
+    (hide (SZ.v bm)) (hide (SZ.v bk)) (hide (SZ.v tile_row)) (hide (SZ.v tile_shared));
+  cp_matrix bm bk #_ #_ tileA sA (get_bdim()) tid;
 
-  let tileB = gpu_matrix_extract_tile' gB bk bn tile_shared tile_col;
+  let tileB = gpu_matrix_extract_tile_ro' gB
+    (hide (SZ.v bk)) (hide (SZ.v bn)) (hide (SZ.v tile_shared)) (hide (SZ.v tile_col));
   cp_matrix bk bn tileB sB (get_bdim()) tid;
 
   ambig_trade_elim ();
@@ -428,7 +433,6 @@ fn populate_shmem
   ();
 }
 
-// #push-options "--debug SMTFail --split_queries always --print_implicits"
 inline_for_extraction noextract
 fn subproducts2d
   (#et : Type0) {| scalar et |}
@@ -487,7 +491,8 @@ fn subproducts2d
           (rAcol |-> vrAcol)
     {
       (* get rid of a few non-linear arithmetic expressions *)
-      let a_tile = gpu_matrix_extract_tile' gA tm 1 arow !dotIdx;
+      let a_tile = gpu_matrix_extract_tile_ro' gA
+        (hide (SZ.v tm)) 1 (hide (SZ.v arow)) (hide (SZ.v !dotIdx));
       let va = gpu_matrix_read a_tile !i0 0sz;
       ambig_trade_elim ();
       rAcol.(!i0) <- va;
@@ -502,7 +507,8 @@ fn subproducts2d
           (i1 |-> vi) **
           (rBrow |-> vrBrow)
     {
-      let b_tile = gpu_matrix_extract_tile' gB 1 tn !dotIdx bcol;
+      let b_tile = gpu_matrix_extract_tile_ro' gB
+        1 (hide (SZ.v tn)) (hide (SZ.v !dotIdx)) (hide (SZ.v bcol));
       let vb = gpu_matrix_read b_tile 0sz !i1;
       ambig_trade_elim ();
       rBrow.(!i1) <- vb;
@@ -562,20 +568,20 @@ fn epilogue
   (tid : szlt (bm/tm * (bn/tn)))
   requires
     gpu **
-    own_thread_tile gC bm bn tm tn bid tid **
+    own_thread_tile gC bm bn tm tn (hide (SZ.v bid)) (hide (SZ.v tid)) **
     (exists* vrchProd.
       pure (Seq.length vrchProd == tm * tn) **
       (rchProd |-> vrchProd))
   ensures
     gpu **
-    own_thread_tile gC bm bn tm tn bid tid **
+    own_thread_tile gC bm bn tm tn (hide (SZ.v bid)) (hide (SZ.v tid)) **
     (exists* vrchProd'.
       pure (Seq.length vrchProd' == tm * tn) **
       (rchProd |-> vrchProd'))
 {
-  unfold own_thread_tile gC bm bn tm tn bid tid;
-  let t_tile = thread_tile (block_tile gC bm bn bid) tm tn tid;
-  assert (rewrites_to t_tile (thread_tile (block_tile gC bm bn bid) tm tn tid));
+  unfold own_thread_tile gC bm bn tm tn (hide (SZ.v bid)) (hide (SZ.v tid));
+  let t_tile = thread_tile (block_tile gC bm bn (hide (SZ.v bid))) tm tn (hide (SZ.v tid));
+  assert (rewrites_to t_tile (thread_tile (block_tile gC bm bn (hide (SZ.v bid))) tm tn (hide (SZ.v tid))));
 
   let mut resIdxM = 0sz;
   while (SZ.(!resIdxM <^ tm))
@@ -615,7 +621,7 @@ fn epilogue
   };
 
   // rewrite each t_tile as thread_tile (block_tile gC bm bn bid) tm tn tid;
-  fold own_thread_tile gC bm bn tm tn bid tid;
+  fold own_thread_tile gC bm bn tm tn (hide (SZ.v bid)) (hide (SZ.v tid));
   ()
 }
 
@@ -757,7 +763,6 @@ fn kf
   ()
 }
 
-#push-options "--z3rlimit 20"
 ghost
 fn setup
   (#et : Type0) {| scalar et |}
@@ -781,6 +786,8 @@ fn setup
   (#_: squash (SZ.fits (rows * cols)))
   (tm : szp{tm /? bm})
   (tn : szp{tn /? bn})
+  (nblk : szp{SZ.v nblk == rows/bm * (cols/bn)})
+  (nthr : szp{SZ.v nthr == bm/tm * (bn/tn)})
   (fA fB : perm)
   ()
   requires
@@ -788,8 +795,8 @@ fn setup
     (gB |-> Frac fB eB) **
     (gC |-> eC)
   ensures
-    (forall+ (bid : natlt (rows/^bm *^ (cols/^bn)))
-             (tid : natlt (bm/^tm *^ (bn/^tn))).
+    (forall+ (bid : natlt nblk)
+             (tid : natlt nthr).
       kpre1 comb gA eA gB eB gC bm bn bk tm tn fA fB bid tid) **
     emp (* frame *)
 {
@@ -821,18 +828,20 @@ fn block_setup
   {| clayout slA, clayout slB |}
   (tm : szp{tm /? bm})
   (tn : szp{tn /? bn})
+  (nblk : szp{SZ.v nblk == rows/bm * (cols/bn)})
+  (nthr : szp{SZ.v nthr == bm/tm * (bn/tn)})
   (fA fB : perm)
   (sh : c_shmems (shmems_desc et bm bn bk))
-  (bid : natlt (rows/^bm *^ (cols/^bn)))
+  (bid : natlt nblk)
   ()
   requires
-    block_setup_tok (bm/^tm *^ (bn/^tn)) **
+    block_setup_tok nthr **
     live_c_shmems sh **
-    (forall+ (tid : natlt (bm/^tm *^ (bn/^tn))).
+    (forall+ (tid : natlt nthr).
       kpre1 comb gA eA gB eB gC bm bn bk tm tn fA fB bid tid)
   ensures
-    block_setup_tok (bm/^tm *^ (bn/^tn)) **
-    (forall+ (tid : natlt (bm/^tm *^ (bn/^tn))).
+    block_setup_tok nthr **
+    (forall+ (tid : natlt nthr).
       kpre comb gA eA gB eB gC bm bn bk slA slB tm tn fA fB sh bid tid) **
     emp (* frame *)
 {
@@ -864,17 +873,19 @@ fn block_teardown
   {| clayout slA, clayout slB |}
   (tm : szp{tm /? bm})
   (tn : szp{tn /? bn})
+  (nblk : szp{SZ.v nblk == rows/bm * (cols/bn)})
+  (nthr : szp{SZ.v nthr == bm/tm * (bn/tn)})
   (fA fB : perm)
   (sh : c_shmems (shmems_desc et bm bn bk))
-  (bid : natlt (rows/^bm *^ (cols/^bn)))
+  (bid : natlt nblk)
   ()
   requires
-    (forall+ (tid : natlt (bm/^tm *^ (bn/^tn))).
+    (forall+ (tid : natlt nthr).
       kpost comb gA eA gB eB gC bm bn bk slA slB tm tn fA fB sh bid tid) **
     emp (* frame *)
   ensures
     live_c_shmems sh **
-    (forall+ (tid : natlt (bm/^tm *^ (bn/^tn))).
+    (forall+ (tid : natlt nthr).
       kpost1 comb gA eA gB eB gC bm bn bk tm tn fA fB bid tid)
 {
   admit();
@@ -901,11 +912,13 @@ fn teardown
   (#_: squash (SZ.fits (bm * bn)))
   (tm : szp{tm /? bm})
   (tn : szp{tn /? bn})
+  (nblk : szp{SZ.v nblk == rows/bm * (cols/bn)})
+  (nthr : szp{SZ.v nthr == bm/tm * (bn/tn)})
   (fA fB : perm)
   ()
   requires
-    (forall+ (bid : natlt (rows/^bm *^ (cols/^bn)))
-             (tid : natlt (bm/^tm *^ (bn/^tn))).
+    (forall+ (bid : natlt nblk)
+             (tid : natlt nthr).
       kpre1 comb gA eA gB eB gC bm bn bk tm tn fA fB bid tid) **
     emp (* frame *)
   ensures
@@ -922,7 +935,6 @@ fn teardown
     // (fun (bid, tid) -> kpost1 comb tile gA gB gC eA eB 1.0R bid tid);
   admit();
 }
-#pop-options
 
 inline_for_extraction noextract
 let mk_kernel
@@ -949,6 +961,8 @@ let mk_kernel
   (tm : szp{tm /? bm})
   (tn : szp{tn /? bn})
   (#fA #fB : perm)
+  (nblk : szp{SZ.v nblk == rows/bm * (cols/bn)})
+  (nthr : szp{SZ.v nthr == bm/tm * (bn/tn)})
   (#_ : squash (SZ.fits (bm*bk + bm/tm*(bn/tn))))
   (#_ : squash (SZ.fits (bk*bn + bm/tm*(bn/tn))))
   (#_ : squash (rows/bm * (cols/bn) <= max_blocks
@@ -958,20 +972,21 @@ let mk_kernel
       ((gA |-> Frac fA eA) ** (gB |-> Frac fB eB) ** (gC |-> eC))
       ((gA |-> Frac fA eA) ** (gB |-> Frac fB eB) ** (gC |-> MS.mmcomb comb eC eA eB))
 = {
-  nblk = rows/^bm *^ (cols/^bn);
-  nthr = (bm /^ tm *^ (bn /^ tn));
+  nblk;// = rows/^bm *^ (cols/^bn);
+  nthr;// = (bm /^ tm *^ (bn /^ tn));
 
   shmems_desc = shmems_desc et bm bn bk;
 
   frame = emp;
-  block_pre  = (fun bid -> forall+ (tid : natlt (bm/^tm *^ (bn/^tn))). kpre1  comb gA eA gB eB gC bm bn bk tm tn fA fB bid tid);
-  block_post = (fun bid -> forall+ (tid : natlt (bm/^tm *^ (bn/^tn))). kpost1 comb gA eA gB eB gC bm bn bk tm tn fA fB bid tid);
-  setup      = setup    comb gA eA gB eB gC eC bm bn bk tm tn fA fB;
-  teardown   = teardown comb gA eA gB eB gC eC bm bn bk tm tn fA fB;
+  block_pre  = (fun bid -> forall+ (tid : natlt nthr). kpre1  comb gA eA gB eB gC bm bn bk tm tn fA fB bid tid);
+  block_post = (fun bid -> forall+ (tid : natlt nthr). kpost1 comb gA eA gB eB gC bm bn bk tm tn fA fB bid tid);
+
+  setup      = setup    comb gA eA gB eB gC eC bm bn bk tm tn nblk nthr fA fB;
+  teardown   = teardown comb gA eA gB eB gC eC bm bn bk tm tn nblk nthr fA fB;
 
   block_frame    = (fun _ar _bid -> emp);
-  block_setup    = block_setup comb gA eA gB eB gC eC bm bn bk slA slB tm tn fA fB;
-  block_teardown = block_teardown comb gA eA gB eB gC eC bm bn bk slA slB tm tn fA fB ;
+  block_setup    = block_setup comb gA eA gB eB gC eC bm bn bk slA slB tm tn nblk nthr fA fB;
+  block_teardown = block_teardown comb gA eA gB eB gC eC bm bn bk slA slB tm tn nblk nthr fA fB ;
 
   kpre      = kpre  comb gA eA gB eB gC bm bn bk slA slB tm tn fA fB;
   kpost     = kpost comb gA eA gB eB gC bm bn bk slA slB tm tn fA fB;
@@ -979,7 +994,6 @@ let mk_kernel
   f = kf comb gA #eA gB #eB gC bm bn bk slA slB tm tn #() #() #fA #fB;
 }
 
-#push-options "--debug SMTFail --split_queries always"
 inline_for_extraction noextract
 fn mmcomb_gpu
   (#et : Type0) {| scalar et |}
@@ -990,11 +1004,11 @@ fn mmcomb_gpu
   (#lC : mlayout rows cols)
   {| clayout lA, clayout lB, clayout lC |}
   (gA : gpu_matrix et lA)
-  (eA : ematrix et rows shared)
+  (#eA : ematrix et rows shared)
   (gB : gpu_matrix et lB)
-  (eB : ematrix et shared cols)
+  (#eB : ematrix et shared cols)
   (gC : gpu_matrix et lC)
-  (eC : ematrix et rows cols)
+  (#eC : ematrix et rows cols)
   (bm : szp{bm /? rows})
   (bn : szp{bn /? cols})
   (bk : szp{bk /? shared})
@@ -1006,19 +1020,18 @@ fn mmcomb_gpu
   (slA : full_mlayout bm bk)
   (slB : full_mlayout bk bn)
   {| clayout slA, clayout slB |}
-  (fA fB : perm)
+  (#fA #fB : perm)
   preserves
     cpu **
-    (gA |-> Frac fA eA) **
-    (gB |-> Frac fB eB)
+    gA |-> Frac fA eA **
+    gB |-> Frac fB eB
   requires
     pure (rows/bm * (cols/bn) <= max_blocks) **
     pure (bm/tm * (bn/tn) <= max_threads) **
-    (gC |-> eC)
+    gC |-> eC
   ensures
     gC |-> MS.mmcomb comb eC eA eB
 {
   (* fixed the inner layouts, or we'd have to propagate this everywhere? *)
-  launch_sync (mk_kernel comb gA gB gC bm bn bk slA slB tm tn ());
+  launch_sync (mk_kernel comb gA gB gC bm bn bk slA slB tm tn (rows/^bm *^ (cols/^bn)) (bm/^tm *^ (bn/^tn)) ());
 }
-
